Test/dafny0/TypeInferenceRefreshErrors.dfy
@@ -1,0 +1,23 @@
+// RUN: %dafny /compile:0 "%s" > "%t"
+// RUN: %diff "%s.expect" "%t"
+
+module Frames {
+  class C {
+    var x: int
+    var y: int
+  }
+
+  // The following was accepted by the old type checking, but it caused a crash in the
+  // translator. Now, we disallow it.
+  function ToC(): C
+  function RegressionTest(): int
+    reads ToC // error: type not allowed: () -> C
+
+  function ToSetReal(): set<real>
+  function ToMap(): map<object, object>
+  function F(r: real, s: set<real>): int
+    reads r // error: not a reference type
+    reads s // error: not a collection of reference type
+    reads ToSetReal // error: not a function to a collection of reference type
+    reads ToMap // error: not a function to a collection of reference type
+}
